theories/Substitution/Introductions/Empty.v
@@ -118,7 +118,7 @@ Section EmptyElimRed.
       + eapply redtm_emptyelim; tea.
         cbn; gen_typing.
     - intros ? [] ?.
-      epose proof (reflect _ (completeness _) _ (wk_id)) as [].
+      epose proof (reflect _ (completeness _)) as [].
       all: repeat rewrite wk_id_ren_on.
       + now eapply ty_emptyElim.
       + now eapply ty_emptyElim.
